UM.v
@@ -111,10 +111,32 @@ destruct H1. simpl in H1. destruct H1. intros.  case A eqn: Ha. simpl in H1. des
 destruct H1. subst m. move /leP in Ha0. simpl. eauto. eapply IHB in H1.
  exact. eauto. eauto. eauto. eauto. destruct H1. } Qed.
  
+Fixpoint replace_column (l:list fill_type)(n:nat):=
+  match l with
+  |nil=>nil
+  |m::l'=> ({|bid_of:= bid_of m ; ask_of:= ask_of m ; tp:=n|})::(replace_column l' n)
+  end.
 
+Lemma replace_column_is_uniform (l: list fill_type)(n:nat):
+  uniform (trade_prices_of (replace_column l n)).
+Proof. { induction l. simpl.  constructor.
+       case l eqn: H. simpl.  constructor. simpl. simpl in IHl. constructor;auto. } Qed.
+
+Lemma last_column_is_trade_price (l:list fill_type)(m:fill_type)(n:nat): In m (replace_column l n)->
+                                                                  (tp m = n).
+Proof. { intro H. induction l. auto. inversion H as [H0 |].  
+inversion H0 as [H1 ]. simpl. exact. apply IHl in H0. exact. } Qed.
+
+Lemma replace_column_elim (l: list fill_type)(n:nat): forall m', In m' (replace_column l n)-> exists m, In m l /\ bid_of m = bid_of m' 
+/\ ask_of m = ask_of m'.
+  Proof. Admitted. 
+  
+
+
+Definition uniform_price B A := bp (bid_of (last (produce_UM B A) m0)).
 
 Definition UM (B:list Bid) (A:list Ask) : (list fill_type) :=
-  replace_column (UM_matching B A)
+  replace_column (produce_UM B A)
                 (uniform_price B A).
 
 
@@ -123,19 +145,350 @@ Theorem UM_is_fair(B: list Bid) (A:list Ask): Is_fair ( UM B A) B A.
 Proof. Admitted.
 
 Theorem UM_is_Ind_Rat (B: list Bid) (A:list Ask):
-  (IsOrd (rev B)) -> (IsOrd A) -> Is_ind_rational (UM B A).
-Proof. { intros HB HA. unfold Is_ind_rational. intros m H. unfold rational. unfold UM in H.
-       replace (trade_price_of m) with (uniform_price B A).
-       assert (H0: exists m', In m' (UM_matching B A) /\ bid_of m' = bid_of m /\ ask_of m' = ask_of m).
+  Sorted by_dbp B -> Sorted by_sp A -> Is_IR (UM B A).
+Proof. { intros HB HA. unfold Is_IR. intros m H. unfold rational. unfold UM in H.
+       replace (tp m) with (uniform_price B A).
+       assert (H0: exists m', In m' (produce_UM B A) /\ bid_of m' = bid_of m /\ ask_of m' = ask_of m).
        apply replace_column_elim with (n:= uniform_price B A). auto.
        destruct H0 as [m' H0]. destruct H0 as [H1 H0]. destruct H0 as [H2 H0].
-       rewrite <- H2. rewrite <- H0. split; apply UP_returns_IR; auto.
-       symmetry; eapply last_column_is_trade_price;eauto.  } Qed.
+       rewrite <- H2. rewrite <- H0. split. admit. (*apply UM_returns_IR*)  auto.
+       admit. admit.  } Admitted.
 
-Theorem UM_is_Uniform (B: list Bid) (A:list Ask) : Is_uniform ( UM B A).
-Proof.  unfold Is_uniform. unfold UM. apply replace_column_is_uniform. Qed.
+Theorem UM_is_Uniform (B: list Bid) (A:list Ask) : Uniform ( UM B A).
+Proof.  unfold Uniform. unfold UM. apply replace_column_is_uniform. Qed.
 
-Theorem UM_is_maximal_Uniform (B: list Bid) (A:list Ask): forall M: list fill_type, Is_uniform M -> |M| <= | (UM B A ) |.
-Proof. Admitted.
+Definition Is_uniform M B A := (Uniform M /\ matching_in B A M /\ Is_IR M).
+
+Lemma matching_on_nilA (B:list Bid) (M:list fill_type) : matching_in B nil M -> M=nil.
+Proof. intros H1. unfold matching_in in H1. destruct H1 as [H1 H2].
+destruct H2 as [H2 H3]. unfold matching in H1. destruct H1 as [H1 H4]. 
+unfold All_matchable in H1. assert (HAMnil: (asks_of M) = nil). eauto.
+Admitted.
+
+Lemma matching_on_nilB (A: list Ask)(M:list fill_type) : matching_in nil A M -> M=nil.
+Proof.  Admitted.
+
+Lemma unmatchableAB_nil (B:list Bid) (A:list Ask) (b:Bid)(a:Ask) (M:list fill_type): Sorted by_dbp (b::B) -> Sorted by_sp (a::A) ->matching_in (b::B) (a::A) M -> b<a-> M=nil.
+Proof.
+  Admitted.
+
+Lemma delete_IR_is_IR (M : list fill_type) (m:fill_type): Is_IR M -> Is_IR (delete m M).
+Proof. unfold Is_IR. eauto. Qed. 
+
+Lemma IR_UM_matchable (M:list fill_type)(b:Bid)(a:Ask): Is_IR M -> Uniform M -> In a (asks_of M) -> In b (bids_of M)->b>=a.
+Proof. { intros H1 H2 Ha Hb. assert (Hm1: exists m1, (In m1 M) /\ a=(ask_of m1)). 
+eauto. assert (Hm2: exists m2, (In m2 M) /\ b=(bid_of m2)). 
+eauto. destruct Hm1 as [m1 Hm1]. destruct Hm2 as [m2 Hm2]. 
+assert (Ht:tp m1 = tp m2). destruct Hm1 as [Hm1m Hm1a]. destruct Hm2 as [Hm2m Hm2b]. eapply Uniform_elim. eauto. all: auto. assert (Hbm: b>= tp m2).
+{ destruct Hm1 as [Hm1m Hm1a]. destruct Hm2 as [Hm2m Hm2b]. subst b.
+eapply H1. exact. } assert (Ham: a<= tp m1). 
+{ destruct Hm1 as [Hm1m Hm1a]. destruct Hm2 as [Hm2m Hm2b]. subst a.
+eapply H1. exact. } omega. } Qed.
+
+
+
+Lemma M'_unifom_ir (M : list fill_type) (m1 m2: fill_type):
+(Is_IR M /\ Uniform M) -> In m1 M -> In m2 M -> 
+Is_IR (({|bid_of:= bid_of m1 ; ask_of:= ask_of m2 ; tp:=(tp m1)|}::delete m1 (delete m2 M))) /\
+Uniform (({|bid_of:= bid_of m1 ; ask_of:= ask_of m2 ; tp:=(tp m1)|}::delete m1 (delete m2 M))).
+Proof. intros H0 H1 H2. split. 
+
+destruct H0 as [H0ir H0uni].  
+set (M'':= delete m1 (delete m2 M)). assert (H_irM'':Is_IR M'').
+subst M''. unfold Is_IR. intros. eauto. assert (Htp: tp m1 = tp m2).
+eauto. assert (Hrationalm2: rational m2). eauto. unfold rational in Hrationalm2. 
+assert (Htpm2: tp m2 >= ask_of m2). eapply Hrationalm2. 
+set (m:={| bid_of := bid_of m1; ask_of := ask_of m2; tp := tp m1 |}).
+assert (mrat:rational m). unfold rational. subst m.  simpl. assert (Hrationalm1: rational m1). eauto. unfold rational in Hrationalm1. 
+assert (Htpm1: bid_of m1 >= tp m1). eapply Hrationalm1. split. eauto. omega. eauto.  
+destruct H0 as [H0ir H0uni].  
+set (M'':= delete m1 (delete m2 M)). assert (H_uniM'':Uniform M'').
+subst M''. eauto. case M'' eqn: HM''. constructor. 
+assert (HeM'': In e M''). rewrite HM''. auto. assert (HeM: In e M).
+eauto.  
+
+assert (H_e: tp e = tp m1). eauto. rewrite <- H_e. eauto. Qed. 
+
+ 
+                 
+                 
+
+Lemma IR_UM_matchable_m (M:list fill_type)(m1 m2:fill_type): Is_IR M -> Uniform M -> In m1 M -> In m2 M-> bid_of m1 >=ask_of m2. 
+Proof. { intros H1 H2 H3 H4. assert (Htp: tp m1 = tp m2). eauto.
+assert (Htpm1b: tp m1 <= bid_of m1). 
+{ unfold Is_IR in H1. unfold rational in H1. eapply H1. exact. }
+assert (Htpm1a: tp m1 >= ask_of m1). 
+{ unfold Is_IR in H1. unfold rational in H1. eapply H1. exact. }
+assert (Htpm2b: tp m2 <= bid_of m2). 
+{ unfold Is_IR in H1. unfold rational in H1. eapply H1. exact. }
+assert (Htpm2a: tp m2 >= ask_of m2). 
+{ unfold Is_IR in H1. unfold rational in H1. eapply H1. exact. }
+omega. } Qed. 
+
+Theorem UM_is_maximal_Uniform (B: list Bid) (A:list Ask)(no_dup_B: NoDup B)(no_dup_A: NoDup A): Sorted by_dbp B -> Sorted by_sp A-> (forall M: list fill_type, Is_uniform M B A-> |M| <= | (produce_UM B A ) |).
+
+Proof. revert B no_dup_B. induction A as [|a A'].
+       { (* base case: when A is nil *)
+         intros B hB H H0.  case B. simpl.
+         { intros M H1. destruct H1 as [H1 H2]. destruct H2 as [H2 H3]. apply matching_on_nilA in H2. subst M. auto. }
+         { intros b l. simpl. intros M H1. destruct H1 as [H1 H2]. destruct H2 as [H2 H3]. apply matching_on_nilA in H2. subst M. auto. } }
+       { (* induction step: when A is a::A' *)
+         intros B hB h h0. case B as [| b B'].
+         { simpl. intros M H1.  destruct H1 as [H1 H2]. destruct H2 as [H2 H3]. apply matching_on_nilB in H2. subst M. auto. }
+         { (*----- induction step : b::B'   and a:: A' ---------*)
+           assert (Case: b < a \/ b >= a ). omega.
+           destruct Case as [C1 | C2].
+                      { (*------C1:  when b and a are not matchable then produce_MM (b::B') A' *)
+             simpl. replace (a <=? b) with false.
+             Focus 2. symmetry. apply /leP. omega. intros M H1.
+             destruct H1 as [H1 H2]. destruct H2 as [H2 H3]. 
+             assert (HM:M=nil). eapply unmatchableAB_nil. eauto. eauto. eauto. exact. subst M. auto. }
+             { (*-- C2: when b and a are matchable then Output is (b,a):: produce_MM B' A'----*)
+             assert (h1: matching_in (b::B') (a::A') (produce_UM (b::B') (a::A'))). {eauto using UP_is_matching. }
+             intros M h2. destruct h2 as [h2a h2]. destruct h2 as [h2 h2b]. 
+              simpl. replace (a <=? b) with true.
+             
+             Focus 2. symmetry. apply /leP. auto.
+             assert (Hb: In b (bids_of M) \/ ~ In b (bids_of M)). eauto.
+             assert (Ha: In a (asks_of M) \/ ~ In a (asks_of M)). eauto.
+             assert (H0: forall M, Is_uniform M B' A' -> |M| <= |(produce_UM B' A')|).
+            
+             { apply IHA'. all: eauto. }
+             destruct Hb as [Hb1 | Hb2]; destruct Ha as [Ha1 | Ha2].
+             { (* Case_ab1: In b (bids_of M) and In a (asks_of M)------*)
+               assert (h3: exists m1, In m1 M /\ a = ask_of m1). eauto.
+               assert (h4: exists m2, In m2 M /\ b = bid_of m2). eauto.
+               destruct h3 as [m1 h3]. destruct h3 as [h3a h3].
+               destruct h4 as [m2 h4]. destruct h4 as [h4a h4].
+               assert (h5: m1 = m2 \/ m1 <> m2). eauto.
+               destruct h5 as [h5a | h5b].
+               { (*-------- h5a : m1 = m2 ---------*)
+                 subst m2. 
+                 set (M' := delete m1 M).  
+                 assert (h5: matching_in B' A' M').
+                 { unfold matching_in. unfold M'. split.
+                   { cut(matching M). auto.  apply h2. } split.
+                   { intros x h5.
+                     assert (h6: In x (b::B')).
+                     { cut (In x (bids_of M)). apply h2.
+                       cut ((delete m1 M) [<=] M). intro h6.
+                       eapply bids_of_intro1. apply h6. all: auto. }
+                     destruct h6 as [h6 | h6].
+                     { absurd (In b (bids_of (delete m1 M))).
+                       subst x. subst b. eauto. subst x;auto. }
+                     { auto. } }
+                    { intros x h5.
+                     assert (h6: In x (a::A')).
+                     { cut (In x (asks_of M)). apply h2.
+                       cut ((delete m1 M) [<=] M). intro h6.
+                       eapply asks_of_intro1. apply h6. all: auto. }
+                     destruct h6 as [h6 | h6].
+                     { absurd (In a (asks_of (delete m1 M))).
+                       subst x. subst a. eauto. subst x;auto. }
+                     { auto. } } } 
+                     assert (h5_ir: Is_IR M'). 
+                     {eapply delete_IR_is_IR. exact. }
+                     assert (h5_unif: Uniform M').
+                     { subst M'. eauto. }
+                     assert (h5_is_uni:Is_uniform M' B' A').
+                     {unfold Is_uniform. eauto. }
+                 assert (h6: |M| = S (|M'|)).
+                 { unfold M'. eauto. }
+                 assert (h7: |M'| <= |(produce_UM B' A')|). apply H0. exact.
+                 simpl. omega. }
+                                { (*-------- h5b : m1 <> m2 ---------*)
+                 set (M'' := delete m1 (delete m2 M)).
+                 assert (h5: |M| = S (S (|M''|))).
+                 { unfold M''.
+                   assert (h3b: In m1 (delete m2 M)).
+                   { auto. }
+                   assert (h6: S (| delete m1 (delete m2 M) |) = |delete m2 M|).
+                   { symmetry. auto. }
+                   rewrite h6. auto. }  
+                 set (m:= {|bid_of:= bid_of m1 ; ask_of:= ask_of m2 ; tp:=(tp m1)|}).
+                 set (M' := (m :: M'')).
+                 
+                 assert (h6: matching_in B' A' M').
+                  { unfold matching_in. split.
+                   { (*----- matching M' ---------------*)
+                     unfold matching. split.
+                     { unfold M'. cut (ask_of m <= bid_of m).
+                       cut (All_matchable M''). auto.
+                       unfold M''. cut (All_matchable M).
+                       auto. eauto. set t:=tp m1.
+                       assert (h_t1:bid_of m1 >=t). 
+                       { subst t. assert ( Hrationalm1:rational m1). eauto.
+                       unfold rational in Hrationalm1. apply Hrationalm1. }
+                       assert (h_t2: t>=ask_of m2).
+                       { subst t. assert ( Hrationalm2:rational m2). eauto.
+                       unfold rational in Hrationalm2. assert (Htpm1m2: tp m1 = tp m2). eauto. rewrite Htpm1m2. apply Hrationalm2. }
+                       simpl. omega. } split.
+                     { (*---- NoDup (bids_of M') ----*)
+                       unfold M'. simpl.
+                       cut (~ In (bid_of m1) (bids_of M'')).
+                       cut (NoDup (bids_of M'')). auto.
+                       { (*--- NoDup (bids_of M'')---*)
+                         cut (matching M''). auto.
+                         unfold M''. eauto. }
+                       { unfold M''. eauto. } }
+                      { (*---- NoDup (asks_of M') ----*)
+                       unfold M'. simpl.
+                       cut (~ In (ask_of m2) (asks_of M'')).
+                       cut (NoDup (asks_of M'')). auto.
+                       { (*--- NoDup (asks_of M'')---*)
+                         cut (matching M''). auto.
+                         unfold M''. eauto. }
+                       { unfold M''.
+                         assert(h6:asks_of(delete m1 (delete m2 M))[<=]asks_of(delete m2 M)).
+                         eauto. intro h7.
+                         absurd (In (ask_of m2) (asks_of (delete m2 M))).
+                         eauto. auto. } } } split. 
+                   { (*----- bids_of M' [<=] B'-------------*)
+                     unfold M'. simpl.
+                     intros x h6. destruct h6 as [h6 | h6].
+                     { cut (In x (b::B')). cut ( x <> b). eauto.
+                       { subst x; subst b. eapply matching_elim14 with (M:= M).
+                         all: auto. eauto. }
+                       { subst x. eapply matching_in_elim4a. apply h2. auto. } }
+                     { unfold M'' in h6.
+                       assert (h7: In x (bids_of M)).
+                       { eauto. }
+                       assert (h8: x <> bid_of m2).
+                       { intro h8. subst x.
+                         assert (h9: In (bid_of m2) (bids_of (delete m2 M))).
+                         eauto.
+                         absurd (In (bid_of m2) (bids_of (delete m2 M))).
+                         eauto. auto. } 
+                       rewrite <- h4 in h8.
+                       assert (h9: In x (b::B')).
+                       { apply h2. auto. }
+                       destruct h9. symmetry in H. contradiction. auto. } } 
+                   { (*------ asks_of M' [<=] A' -------*)
+                     unfold M'. simpl.
+                     intros x h6. destruct h6 as [h6 | h6].
+                     { cut (In x (a::A')). cut ( x <> a). eauto.
+                       { subst x; subst a. eapply matching_elim15 with (M:= M).
+                         all: auto. eauto. }
+                       { subst x. eapply matching_in_elim5a. apply h2. auto. } }
+                     { unfold M'' in h6.
+                       assert (h7: In x (asks_of M)).
+                       { eauto. } 
+                       assert (h8: x <> ask_of m1).
+                       { intro h8. subst x.
+                         assert (h9: In (ask_of m1) (asks_of (delete m2 M))).
+                         eauto.
+                         absurd (In (ask_of m1) (asks_of (delete m1 (delete m2 M)))).
+                         eauto. auto. }
+                       rewrite <- h3 in h8.
+                       assert (h9: In x (a::A')).
+                       { apply h2. auto. }
+                       destruct h9. symmetry in H. contradiction. auto. } } }          
+
+                     assert (h5_is_uni: (Is_IR M') /\ (Uniform M')).
+                     subst M'. subst M''. subst m. 
+                     assert (h_temp1: (Is_IR M /\ Uniform M) ). auto. 
+                     eapply M'_unifom_ir with 
+                     (M:=M) (m1:=m1) (m2:=m2). exact. exact. exact.
+                      
+                       assert (h5_ir: Is_IR M'). 
+                     { apply h5_is_uni.  }
+                       assert (h5_unif: Uniform M'). 
+                     { apply h5_is_uni.  }
+                      (*continue from here*) 
+                    
+                     assert (h5_is_unif:Is_uniform M' B' A').
+                     {unfold Is_uniform. eauto. }
+                     
+             assert (h7: |M'| <= |(produce_UM B' A')|). apply H0. exact.
+                 unfold M' in h7. simpl in h7. rewrite h5. simpl. omega. } }
+             { (* Case_ab2: In b (bids_of M) and ~ In a (asks_of M)----*)
+               assert (h3: exists m, In m M /\ b = bid_of m). eauto.
+               destruct h3 as [m h3]. destruct h3 as [h3a h3].
+               set (M' := delete m M).
+               assert (h4: matching_in B' A' M').
+               { unfold matching_in. split.
+                 { (*------ matching M' -----------*)
+                   unfold M'. eauto. } split.
+                 { (*------bids_of M' [<=] B'------*)
+                   intros x h4.
+                   assert (h5: In x (bids_of M)).
+                   { unfold M' in h4. eauto. }
+                   assert (h5a: In x (b::B')).
+                   { apply h2. auto. }
+                   assert (h6: x <> b).
+                   { intro h6. unfold M' in h4.
+                     subst x;subst b.
+                     absurd (In (bid_of m) (bids_of (delete m M))).
+                     eauto. auto. }
+                   eapply in_inv2. all: eauto. }
+                 { (*------ asks_of M' [<=] A'-------*)
+                   intros x h4.
+                   assert (h5: In x (asks_of M)).
+                   { unfold M' in h4. eauto. }
+                   assert (h6: x <> a).
+                   { intro h6. subst x. contradiction. }
+                   assert (h7: In x (a::A')).
+                   { apply h2. auto. }
+                   eapply in_inv2. all: eauto.  } }
+               assert (h5: |M| = S (|M'|)).
+               { unfold M'. eauto. }
+                assert (h5_ir: Is_IR M'). 
+                     { subst M'. eapply Is_IR_elim2. exact. }
+                     assert (h5_unif: Uniform M').
+                     { subst M'.  eauto. }
+                     assert (h5_is_uni:Is_uniform M' B' A').
+                     {unfold Is_uniform. eauto. }
+               assert (h6: |M'| <= |(produce_UM B' A')|). apply H0. exact.
+               simpl. omega. }
+             { (* Case_ab3: ~ In b (bids_of M) and In a (asks_of M)----*)
+               assert (h3: exists m, In m M /\ a = ask_of m). eauto.
+               destruct h3 as [m h3]. destruct h3 as [h3a h3].
+               set (M' := delete m M).
+               
+               assert (h4: matching_in B' A' M').
+               { unfold matching_in. split.
+                 { (*------ matching M' -----------*)
+                   unfold M'. eauto. } split.
+                 { (*------bids_of M' [<=] B'------*)
+                   intros x h4.
+                   assert (h5: In x (bids_of M)).
+                   { unfold M' in h4. eauto. }
+                   assert (h6: x <> b).
+                   { intro h6. subst x. contradiction. }
+                   assert (h7: In x (b::B')).
+                   { apply h2. auto. }
+                   eapply in_inv2. all: eauto. }
+                 { (*------ asks_of M' [<=] A'-------*)
+                   intros x h4.
+                   assert (h5: In x (asks_of M)).
+                   { unfold M' in h4. eauto. }
+                   assert (h5a: In x (a::A')).
+                   { apply h2. auto. }
+                   assert (h6: x <> a).
+                   { intro h6. unfold M' in h4.
+                     subst x;subst a.
+                     absurd (In (ask_of m) (asks_of (delete m M))).
+                     eauto. auto. }
+                   eapply in_inv2. all: eauto. } } 
+               assert (h5: |M| = S (|M'|)).
+               { unfold M'. eauto. }
+                assert (h5_ir: Is_IR M'). 
+                     { subst M'. eapply Is_IR_elim2. exact. }
+                     assert (h5_unif: Uniform M').
+                     { subst M'. eauto. }
+                     assert (h5_is_uni:Is_uniform M' B' A').
+                     {unfold Is_uniform. eauto. }
+               assert (h6: |M'| <= |(produce_UM B' A')|). apply H0. exact.
+               simpl. omega. }
+             { (* Case_ab4: ~ In b (bids_of M) and ~ In a (asks_of M)---*)
+               assert (h3: matching_in B' A' M). eauto using matching_in_elim8.
+                assert (h5_ir: Is_IR M). 
+                     { exact. }
+                     assert (h5_unif: Uniform M).
+                     {exact. }
+                     assert (h5_is_uni:Is_uniform M B' A').
+                     {unfold Is_uniform. eauto. }
+               cut (|M| <= | produce_UM B' A'|). simpl. omega. apply H0. exact. }   } } } Qed.  
+               
 
 End UM.
